Make names more understandable

CCFPQ/CCFPQ_Result.v
@@ -12,16 +12,16 @@ Set Strict Implicit.
 (* The main goal is to show that 3 sematics of CCFPQ evaluation can be *)
 (* derived from parse tree of a graph.                                 *)
 
-Inductive Parse_tree : Grammar -> V_set -> A_set -> Vertex ->
+Inductive Parse_tree : Grammar -> Vertex_set -> Arc_set -> Vertex ->
                        Vertex -> var -> Prop :=
-  | Leaf : forall (g : Grammar) (V : V_set) (A : A_set) (x1 x2 : Vertex)
+  | Leaf : forall (g : Grammar) (V : Vertex_set) (A : Arc_set) (x1 x2 : Vertex)
                   (v : var) (t : ter),
       V x1 -> V x2 -> In (Rt v t) g -> A (A_ends x1 x2 t) ->
         Parse_tree g V A x1 x2 v
-  | Empty_leaf : forall (g : Grammar) (V : V_set) (A : A_set) (x : Vertex)
+  | Empty_leaf : forall (g : Grammar) (V : Vertex_set) (A : Arc_set) (x : Vertex)
                         (v : var) (e : eps),
       V x -> In (Re v e) g -> Parse_tree g V A x x v
-  | Node : forall (g : Grammar) (V : V_set) (A : A_set) (x1 x2 x3 : Vertex)
+  | Node : forall (g : Grammar) (V : Vertex_set) (A : Arc_set) (x1 x2 x3 : Vertex)
                   (v v1 v2 : var),
       V x1 -> V x2 -> V x3 -> In (Rv v v1 v2) g ->
         Parse_tree g V A x1 x2 v1 -> Parse_tree g V A x2 x3 v2 ->
@@ -29,23 +29,23 @@ Inductive Parse_tree : Grammar -> V_set -> A_set -> Vertex ->
 
 (* First semantic is relation. *)
 
-Inductive Derivability_relation : Grammar -> V_set -> A_set ->
+Inductive Derivability_relation : Grammar -> Vertex_set -> Arc_set ->
                                   Vertex -> Vertex -> var -> Prop :=
-  | Empty_rule : forall (g : Grammar) (V : V_set) (A : A_set) (x: Vertex)
+  | Empty_rule : forall (g : Grammar) (V : Vertex_set) (A : Arc_set) (x: Vertex)
                         (v: var) (e: eps),
        V x -> In (Re v e) g -> Derivability_relation g V A x x v
-  | Arc_with_ter_label : forall (g : Grammar) (V : V_set) (A : A_set)
+  | Arc_with_ter_label : forall (g : Grammar) (V : Vertex_set) (A : Arc_set)
                                 (x1 x2 : Vertex) (v : var) (t : ter),
        V x1 -> V x2 -> In (Rt v t) g -> A (A_ends x1 x2 t) ->
          Derivability_relation g V A x1 x2 v
-  | Rule_application : forall (g : Grammar) (V : V_set) (A : A_set)
+  | Rule_application : forall (g : Grammar) (V : Vertex_set) (A : Arc_set)
                        (x1 x2: Vertex) (v v1 v2 : var),
        (exists (x' : Vertex), V x1 -> V x2 -> V x' -> In (Rv v v1 v2) g ->
          Derivability_relation g V A x1 x' v1 /\
            Derivability_relation g V A x' x2 v2) ->
        Derivability_relation g V A x1 x2 v.
 
-Theorem Parse_tree_to_relation : forall (g : Grammar) (V : V_set) (A : A_set)
+Theorem Parse_tree_to_relation : forall (g : Grammar) (V : Vertex_set) (A : Arc_set)
                                         (x1 x2 : Vertex) (v : var),
         Parse_tree g V A x1 x2 v -> Derivability_relation g V A x1 x2 v.
 Proof.
@@ -96,19 +96,19 @@ Qed.
 Definition get_labels_from_walk x1 x2 vl al (walk : D_walk x1 x2 vl al)
            : list ter := get_labels al.
 
-Inductive Single_path_semantics : forall (g : Grammar) (V : V_set) (A : A_set)
+Inductive Single_path_semantics : forall (g : Grammar) (V : Vertex_set) (A : Arc_set)
             (v : var) (x1 x2 : Vertex) (vl : list Vertex) (al : list Arc),
           D_walk x1 x2 vl al -> Prop :=
-  | Empty_path : forall (g : Grammar) (V : V_set) (A : A_set) (x : Vertex)
+  | Empty_path : forall (g : Grammar) (V : Vertex_set) (A : Arc_set) (x : Vertex)
                         (v : var) (e : eps),
       V x -> In (Re v e) g ->
         Single_path_semantics g V A v x x V_nil A_nil (DW_null x)
-  | One_arc_path : forall (g : Grammar) (V : V_set) (A : A_set)
+  | One_arc_path : forall (g : Grammar) (V : Vertex_set) (A : Arc_set)
                           (x1 x2 : Vertex) (v : var) (t : ter),
       V x1 -> V x2 -> In (Rt v t) g -> A (A_ends x1 x2 t) ->
         Single_path_semantics g V A v x1 x2 [x2] [A_ends x1 x2 t]
           (DW_step x1 x2 x2 V_nil A_nil t (DW_null x2))
-  | Combine_path : forall (g : Grammar) (V : V_set) (A : A_set)
+  | Combine_path : forall (g : Grammar) (V : Vertex_set) (A : Arc_set)
                (x1 x2 x3 : Vertex) (v v1 v2 : var)
                (al1 al2 : list Arc) (vl1 vl2 : list Vertex)
                (dw1 : D_walk x1 x2 vl1 al1) (dw2 : D_walk x2 x3 vl2 al2),
@@ -134,7 +134,7 @@ Proof.
     done.
 Qed.
 
-Theorem Derives_single_path : forall (g : Grammar) (V : V_set) (A : A_set)
+Theorem Derives_single_path : forall (g : Grammar) (V : Vertex_set) (A : Arc_set)
             (v : var) (x1 x2 : Vertex) (vl : list Vertex) (al : list Arc)
             (dw : D_walk x1 x2 vl al)
             (p : Single_path_semantics g V A v x1 x2 vl al dw),
@@ -161,8 +161,8 @@ Proof.
     done.
 Qed.
 
-Theorem Parse_tree_to_single_path : forall (g : Grammar) (V : V_set)
-    (A : A_set) (x1 x2 : Vertex) (v : var),
+Theorem Parse_tree_to_single_path : forall (g : Grammar) (V : Vertex_set)
+    (A : Arc_set) (x1 x2 : Vertex) (v : var),
     Parse_tree g V A x1 x2 v ->
       exists (vl : list Vertex) (al : list Arc) (dw : D_walk x1 x2 vl al),
         Single_path_semantics g V A v x1 x2 vl al dw.
@@ -173,31 +173,19 @@ Proof.
   + exists [x2],
            [A_ends x1 x2 t],
            (DW_step x1 x2 x2 V_nil A_nil t (DW_null x2)).
-    apply One_arc_path.
-    done.
-    done.
-    done.
-    done.
+    by apply: One_arc_path.
 
   + exists [],
            [],
            (DW_null x).
-    apply: Empty_path.
-    done.
-    done.
+    by apply: Empty_path.
 
   + destruct IHpt1 as [vl1 [al1 [dw1 IHpt1]]].
     destruct IHpt2 as [vl2 [al2 [dw2 IHpt2]]].
     exists (vl1 ++ vl2),
            (al1 ++ al2),
            (D_walk_append x1 x2 x3 vl1 vl2 al1 al2 dw1 dw2).
-    apply: Combine_path.
-    done.
-    done.
-    done.
-    exact H2.
-    done.
-    done.
+    apply: Combine_path; eauto.
 Qed.
 
 (* Third semantic is all paths. *)
@@ -214,16 +202,16 @@ Fixpoint get_all_pairs (all1 all2 : list (list Arc)) : list (list Arc) :=
     | l::t => (get_pairs l all2) ++ (get_all_pairs t all2)
   end.
 
-Inductive All_path_semantics : forall (g : Grammar) (V : V_set) (A : A_set)
+Inductive All_path_semantics : forall (g : Grammar) (V : Vertex_set) (A : Arc_set)
           (v : var) (x1 x2 : Vertex) (all : list (list Arc)), Prop :=
-  | Empty_paths : forall (g : Grammar) (V : V_set) (A : A_set) (x : Vertex)
+  | Empty_paths : forall (g : Grammar) (V : Vertex_set) (A : Arc_set) (x : Vertex)
                          (v : var) (e : eps),
       V x -> In (Re v e) g -> All_path_semantics g V A v x x [[]]
-  | One_arc_paths : forall (g : Grammar) (V : V_set) (A : A_set)
+  | One_arc_paths : forall (g : Grammar) (V : Vertex_set) (A : Arc_set)
                            (x1 x2 : Vertex) (v : var) (t : ter),
       V x1 -> V x2 -> In (Rt v t) g -> A (A_ends x1 x2 t) ->
         All_path_semantics g V A v x1 x2 [[A_ends x1 x2 t]]
-  | Combine_paths : forall (g : Grammar) (V : V_set) (A : A_set)
+  | Combine_paths : forall (g : Grammar) (V : Vertex_set) (A : Arc_set)
                            (x1 x2 x3 : Vertex) (v v1 v2 : var)
                            (all1 all2 : list (list Arc)),
       V x1 -> V x2 -> V x3 -> In (Rv v v1 v2) g ->
@@ -231,8 +219,8 @@ Inductive All_path_semantics : forall (g : Grammar) (V : V_set) (A : A_set)
           All_path_semantics g V A v2 x2 x3 all2 ->
             All_path_semantics g V A v x1 x3 (get_all_pairs all1 all2).
 
-Theorem Parse_tree_to_all_path : forall (g : Grammar) (V : V_set)
-    (A : A_set) (x1 x2 : Vertex) (v : var),
+Theorem Parse_tree_to_all_path : forall (g : Grammar) (V : Vertex_set)
+    (A : Arc_set) (x1 x2 : Vertex) (v : var),
     Parse_tree g V A x1 x2 v ->
       exists (all : list (list Arc)), All_path_semantics g V A v x1 x2 all.
 Proof.
@@ -458,7 +446,7 @@ Proof.
     done.
 Qed.
 
-Theorem derives_all_path : forall (g : Grammar) (V : V_set) (A : A_set)
+Theorem derives_all_path : forall (g : Grammar) (V : Vertex_set) (A : Arc_set)
          (v : var) (x1 x2 : Vertex) (all : list (list Arc))
          (aps : All_path_semantics g V A v x1 x2 all),
          forall (al : list Arc), In al all -> Der_ter_list g v (get_labels al).
